theories/StackMachines/Util/List_facts.v
@@ -3,7 +3,7 @@ Import ListNotations.
 
 Require Import Undecidability.StackMachines.Util.Nat_facts.
 
-From Coq Require Import ssreflect ssrbool ssrfun.
+Require Import ssreflect ssrbool ssrfun.
 
 Lemma seq_last {m n} : seq m (1+n) = seq m n ++ [m + n].
 Proof. have -> : 1+n = n+1 by lia. by rewrite seq_app. Qed.
